WIP

HappensBefore.v
@@ -2,31 +2,70 @@ From Coq Require Import Lists.List.
 
 From Elo Require Import Core.
 
+Notation "'<<' ev1 ',' tc ',' ev2 '>>'" := (ev2 :: tc +++ ev1).
+
+(* ------------------------------------------------------------------------- *)
+(* is-acquire & is-release                                                   *)
+(* ------------------------------------------------------------------------- *)
+
+Definition is_acquire (ad : addr) (e : eff) :=
+  (exists t, e = e_acq ad t) \/ e = e_wacq ad.
+
+Definition is_release (ad : addr) (e : eff) :=
+  e = e_rel ad \/ e = e_wrel ad.
+
+Lemma isacquire_dec : forall ad e,
+  Decidable.decidable (is_acquire ad e).
+Proof.
+  unfold Decidable.decidable. unfold not. unfold is_acquire. intros.
+  rename ad into ad'. destruct e;
+  try solve [right; intros [[? F] | F]; invc F];
+  nat_eq_dec ad' ad;
+  try solve [right; intros [[? F] | F]; invc F; congruence];
+  eauto.
+Qed.
+
+(* ------------------------------------------------------------------------- *)
+(* happens-before                                                            *)
+(* ------------------------------------------------------------------------- *)
+
 Inductive happens_before : trace -> Prop :=
-  | hb_tid : forall tc tid e1 e2,
+  | hb_thread : forall tc tid e1 e2,
     happens_before ((tid, e2) :: tc +++ (tid, e1))
 
-  | hb_rel_acq : forall tc tid1 tid2 ad t,
-    happens_before ((tid2, e_acq ad t) :: tc +++ (tid1, e_rel ad))
+  | hb_release_acquire : forall tc tid1 tid2 ad e1 e2,
+    is_release ad e1 ->
+    is_acquire ad e2 ->
+    happens_before ((tid2, e2) :: tc +++ (tid1, e1))
 
-  | hb_wrel_acq : forall tc tid1 tid2 ad t,
-    happens_before ((tid2, e_acq ad t) :: tc +++ (tid1, e_wrel ad))
+  | hb_initialize_acquire : forall tc tid1 tid2 ad t e,
+    is_acquire ad e ->
+    happens_before ((tid2, e) :: tc +++ (tid1, e_init ad t))
 
-  | hb_rel_wacq : forall tc tid1 tid2 ad,
-    happens_before ((tid2, e_wacq ad) :: tc +++ (tid1, e_rel ad))
-
-  | hb_wrel_wacq : forall tc tid1 tid2 ad,
-    happens_before ((tid2, e_wacq ad) :: tc +++ (tid1, e_wrel ad))
-
-  | hb_init_acq : forall tc tid1 tid2 ad t1 t2,
-    happens_before ((tid2, e_acq ad t2) :: tc +++ (tid1, e_init ad t1))
-
-  | hb_init_wacq : forall tc tid1 tid2 ad t,
-    happens_before ((tid2, e_wacq ad) :: tc +++ (tid1, e_init ad t))
-
-  | hb_trans : forall tcA tcB ev1 ev2 ev3,
+  | hb_transitivity : forall tcA tcB ev1 ev2 ev3,
     happens_before (ev2 :: tcA +++ ev1) ->
     happens_before (ev3 :: tcB +++ ev2) ->
     happens_before (ev3 :: tcB ++ ev2 :: tcA +++ ev1)
   .
+
+(* lemmas ------------------------------------------------------------------ *)
+
+Lemma happens_before_from_initialize_acquire_effects :
+  forall tc tc1 tc2 tc3 tid1 tid2 e1 e2 eAcq eInit ad t,
+    is_acquire ad eAcq  ->
+    eInit = e_init ad t ->
+    tc = (tc3 ++ (tid2, eAcq) :: tc2 ++ (tid1, eInit) :: tc1) ->
+    happens_before <<(tid1, e1), tc, (tid2, e2)>>.
+Proof.
+  intros * ? ? Htc.
+  rewrite app_comm_cons in Htc. rewrite app_assoc in Htc.
+  remember (tc3 ++ (tid2, eAcq) :: tc2) as tc' eqn: Htc'.
+  rewrite Htc. clear Htc.
+  unfold add. rewrite <- app_assoc. rewrite <- app_comm_cons.
+  eapply hb_transitivity; eauto using happens_before.
+  rewrite Htc'. clear Htc'.
+  unfold add. rewrite <- app_assoc. rewrite <- app_comm_cons.
+  subst.
+  eapply hb_transitivity; eauto using happens_before.
+Qed.
 
